Calculator/CalcAlternative.lean
@@ -3,98 +3,195 @@ import Calculator.Calculator
 
 namespace Tactic.Calculation.Alternate
 
-open Lean Meta Elab Term Macro Command Tactic
+open Lean Meta Elab Term Tactic Parser Tactic Command
 
-syntax step := term " by " Parser.Tactic.tacticSeqIndentGt
-syntax steps := ppLine ppIndent(atomic(step)*)
-syntax finalStep := ppLine ppIndent(term)
-syntax "calcs" steps finalStep " ∎"? : tactic
+open Tactic.Calculation.Alternate
 
-def unpkgCalcStep (step : TSyntax ``step) : TermElabM (Term × Term) :=
-  match step with
-  | `(step| $t:term by $w) => return (t, <- `(by $w))
-  | _ => throwUnsupportedSyntax
+-- partial def finishExplanationBlock (nesting : Nat) : ParserFn := fun c s =>
+--   let i := s.pos
+--   if h : c.atEnd i then eoi s
+--   else
+--     let curr := c.get' i h
+--     let i    := c.next' i h
+--     if curr == '-' then
+--       if h : c.atEnd i then eoi s
+--       else
+--         let curr := c.get' i h
+--         if curr == '}' then -- "-/" end of comment
+--           if nesting == 1 then s.next' c i h
+--           else finishExplanationBlock (nesting-1) c (s.next' c i h)
+--         else
+--           finishExplanationBlock nesting c (s.setPos i)
+--     else if curr == '{' then
+--       if h : c.atEnd i then eoi s
+--       else
+--         let curr := c.get' i h
+--         if curr == '-' then finishExplanationBlock (nesting+1) c (s.next' c i h)
+--         else finishExplanationBlock nesting c (s.setPos i)
+--     else finishExplanationBlock nesting c (s.setPos i)
+-- where
+--   eoi s := s.mkUnexpectedError (pushMissing := true) "unterminated comment"
 
-def mkCalcStepView (step : TSyntax ``step) : TermElabM CalcStepView :=
-  withRef step do
+-- def explanationBody : Parser := {
+--   fn := rawFn (finishExplanationBlock 1) (trailingWs := true)
+-- }
+
+-- @[combinator_parenthesizer explanationBody, expose]
+-- def explanationBody.parenthesizer := PrettyPrinter.Parenthesizer.visitToken
+-- @[combinator_formatter explanationBody, expose]
+-- def explanationBody.formatter := PrettyPrinter.Formatter.visitAtom Name.anonymous
+
+declare_syntax_cat relOp
+declare_syntax_cat relStep
+
+syntax "step_by " relOp "[" term "," term "]" : relStep
+
+syntax justification :=
+  interpolatedStr(term)?
+  ppSpace ("by " tacticSeqIndentGt)
+
+syntax step := relOp justification ppLine colEq term:51
+
+syntax "calculator" ppLine withPosition(term:51 (ppLine step)*)
+  : tactic
+
+syntax unicode(" = ", " ≡ ") : relOp
+syntax unicode(" <- ", " ← ") : relOp
+syntax unicode(" -> ", " → ") : relOp
+
+syntax "rel[" relOp "]" : term
+
+def implies (p q) := p → q
+
+macro_rules
+  | `(relStep| step_by = [$lhs, $rhs]) => `($lhs = $rhs)
+  | `(relStep| step_by → [$lhs, $rhs]) => `(implies $lhs $rhs)
+  | `(relStep| step_by ← [$lhs, $rhs]) => `(implies $rhs $lhs)
+
+open TSyntax Compat in
+def mkCalcStepViews (fst : Term) (steps : Array (TSyntax ``step))
+    : TermElabM (Array CalcStepView) := do
+  let mut views : Array CalcStepView <- withRef fst do
+    let term <- `($fst = _)
+    let proof <- `(rfl)
+    pure #[{ ref := fst, term, proof }]
+  for step in steps do
     match step with
-    | `(step| $t:term by $w:tactic) => return { ref := step, term := t, proof := <- `(by { $w }) }
+    | `(step| $rel $[$comment]? by $tac $rhs) => do
+      let relExp <- withRef step do
+        liftMacroM (expandMacros (<- `(relStep| step_by $rel [_, $rhs])))
+      match relExp with
+      | `(term| $relFn) => do
+        let proof <- withRef tac `(by $tac)
+        views := views.push { ref := step, term := relFn, proof }
     | _ => throwUnsupportedSyntax
+  return views
 
-def mkCalcStepViews (steps : TSyntax ``steps) (last : Term)
-  : TermElabM (Array CalcStepView) :=
-  match steps with
-  | `(steps| $fst $rest*) => do
-    let mut (t1, prf) <- unpkgCalcStep fst
-    let mut steps := #[{ ref := fst, term := <- `($t1 = _), proof := <- ``(rfl) }]
-    for step in rest do
-      let `(step| $t by $w) := step | throwUnsupportedSyntax
-      steps := steps.push { ref := step, term := t, proof := prf }
-      prf <- `(by $w)
-    steps := steps.push { ref := last, term := last, proof := prf }
-    return steps
-  | _ => throwUnsupportedSyntax
+def sendWidgetInfo (step : CalcStepView) (tmIndent relIndent : Nat) : TacticM Unit := do
+  let some range := (<- getFileMap).lspRangeOfStx? step.ref | return
+  let json := json% {
+    "isFirst": false,
+    "replaceRange": $({ range with start := { range.start with character := relIndent } }),
+    "indent": $tmIndent,
+    "relIndent": $relIndent,
+    "altStyle": true
+  }
+  match step.ref with
+  | `(step| $_rel $[$comment]? by $tac $rhs) => do
+    let _ <- Term.elabTerm rhs none
+    Widget.savePanelWidgetInfo panel.javascriptHash (pure json) tac
+  | _ => return ()
 
 elab_rules : tactic
-| `(tactic|calcs%$tk $steps $last:term $[∎]?) => withRef tk do
+| `(tactic|calculator%$tk $fst:term $steps:step*) => withRef tk do
   Tactic.closeMainGoalUsing `calc (checkNewUnassigned := false) fun target tag => do
-    Tactic.withTacticInfoContext steps do
-      let steps <- mkCalcStepViews steps last
-      let target := (<- instantiateMVars target).consumeMData
-      let (val, mvarIds) <- Tactic.withCollectingNewGoalsFrom
-        (parentTag := tag) (tagSuffix := `calcs)
+    Tactic.withTacticInfoContext tk do
+      let stepViews ← mkCalcStepViews fst steps
+      -- Send info to widget to render suitable calculation suggestions for each step
+      let mut lhs := fst
+      let some lhsRange := (<- getFileMap).lspRangeOfStx? lhs | throwUnsupportedSyntax
+      for view in stepViews do
+        match view.ref with
+        | `(step| $rel $[$comment]? by $_tac $rhs) => do
+          let some relRange := (<- getFileMap).lspRangeOfStx? rel | throwUnsupportedSyntax
+          sendWidgetInfo view lhsRange.start.character relRange.start.character
+          lhs := rhs
+        | _ => continue -- First line
+      -- Process all of the steps
+      let target := (← instantiateMVars target).consumeMData
+      let (val, mvarIds) ← Tactic.withCollectingNewGoalsFrom
+        (parentTag := tag) (tagSuffix := `calculator)
         <| Tactic.runTermElab do
-        let (val, valType) <- Term.elabCalcSteps steps
-        if (<- isDefEq valType target) then
-          -- Immediately the right type, no need for further processing.
+        let (val, valType) ← Term.elabCalcSteps stepViews
+        if (← isDefEq valType target) then
+          -- If the produced proof value is of the correct type already, then just
+          -- return it immediately.
           return val
-        let some (_, lhs, rhs) <- Term.getCalcRelation? valType | unreachable!
-        if let some (er, elhs, erhs) <- Term.getCalcRelation? target then
-          -- Feature: if the goal is `x ~ y`, try extending the `calc` with `_ ~ y` with a
-          -- new "last step" goal.
-          if <- isDefEq lhs elhs <&&> isDefEq (<- inferType rhs) (<- inferType elhs) then
+        -- Otherwise, try to synthesise a final unifying step
+        let some (_rel, lhs, rhs) ← Term.getCalcRelation? valType | unreachable!
+        if let some (er, elhs, erhs) ← Term.getCalcRelation? target then
+          if ← isDefEq lhs elhs <&&> isDefEq (← inferType rhs) (← inferType elhs) then
             let lastStep := mkApp2 er rhs erhs
-            let lastStepGoal <- mkFreshExprSyntheticOpaqueMVar lastStep (tag := tag ++ `calc.step)
+            let lastStepGoal ← mkFreshExprSyntheticOpaqueMVar lastStep (tag := tag ++ `calc.step)
             try
-              let (val', valType') <- Term.mkCalcTrans val valType lastStepGoal lastStep
-              if (<- isDefEq valType' target) then
+              let (val', valType') ← Term.mkCalcTrans val valType lastStepGoal lastStep
+              if (← isDefEq valType' target) then
                 return val'
             catch _ =>
               pure ()
         -- Calc extension failed, so let's go back and mimic the `calc` expression
         Term.ensureHasTypeWithErrorMsgs target val
-          (mkImmedErrorMsg := fun _ => Term.throwCalcFailure steps)
-          (mkErrorMsg := fun _ => Term.throwCalcFailure steps)
+          (mkImmedErrorMsg := fun _ => Term.throwCalcFailure stepViews)
+          (mkErrorMsg := fun _ => Term.throwCalcFailure stepViews)
       pushGoals mvarIds
       return val
 
-section Testing
+elab stx:"calculator?" rel:relOp : tactic => Tactic.withMainContext do
+  let (_rel, lhs, rhs) <- getCalcRelation
+  let s <- `(tactic| calculator
+  $(<- Lean.PrettyPrinter.delab lhs)
+    = by todo
+  $(<- Lean.PrettyPrinter.delab rhs))
+  Tactic.TryThis.addSuggestions stx #[.suggestion s] (header := "Create calculator tactic:")
+  Tactic.evalTactic (<- `(tactic|sorry))
 
-open Tactic.Calculation
+-- @[simp]
+-- def rev {a} : List a → List a
+--   | [] => []
+--   | x :: xs => rev xs ++ [x]
 
-@[simp]
-def rev {a} : List a → List a
-  | [] => []
-  | x :: xs => rev xs ++ [x]
+-- structure RevSpec a : Type where
+--   fastrev : List a -> List a -> List a
+--   correct : ∀ xs ys, rev xs ++ ys = fastrev xs ys
 
-structure RevSpec a : Type where
-  fastrev : List a -> List a -> List a
-  correct : ∀ xs ys, rev xs ++ ys = fastrev xs ys
+-- def eg : 1 = 1 := by
+--   calculator
+--     1
 
-def revCalc {a} : RevSpec a := by
-  calculate fastrev
-  refine fastrev => apply List.rec
-  intro xs
-  induction xs <;> intro ys
-  case nil =>
-    calcs
-      (rev [] ++ ys)
-        by rfl
-      (_ = ys)
-        by define fastrev [] ys := ys
-      (_ = fastrev [] ys)
+-- def revCalc {a} : RevSpec a := by
+--   calculate fastrev
+--   give fastrev by recursion
+--   intro xs
+--   (induction xs) <;> intro ys
+--   case nil =>
+--     calculator
+--     rev [] ++ ys
+--       = by rfl
+--     ys
+--       = by give fastrev [] ys := ys
+--     fastrev [] ys
+--   case cons x xs ih => calculator
+--       rev (x :: xs) ++ ys
+--     = by simp only [rev]
+--       rev xs ++ [x] ++ ys
+--     = by simp only [List.append_assoc]
+--       rev xs ++ ([x] ++ ys)
+--     = by rfl
+--       rev xs ++ x :: ys
+--     = by rw [ih]
+--       fastrev xs (x :: ys)
+--     = by give fastrev (x :: xs) ys := fastrev xs (x :: ys)
+--       fastrev (x :: xs) ys
 
-
-end Testing
 
 end Tactic.Calculation.Alternate
