Example/ExampleAlternative.lean
@@ -1,0 +1,218 @@
+import Calculator.Calculator
+import Calculator.CalcAlternative
+import Mathlib.Tactic.Common
+import Mathlib.Data.List.Basic
+import Mathlib.Data.Nat.Basic
+import Mathlib.Util.CompileInductive
+
+namespace Calculator.Example.Alternative
+
+open Tactic.Calculation
+open Tactic.Calculation.Alternate
+
+open List
+
+/-
+
+Want to be able to introduce "global" let-bindings during calculations.
+
+So like,
+
+calculator
+  exec c (eval (add x y) :: s)
+    = by rfl
+  exec c ((eval x + eval y) :: s)
+    = by let m = eval x; let n = eval y
+  exec c ((m + n) :: s)
+    ...
+-/
+
+def f {a b} : (a × b) -> (b × a) := by calculator
+  (a × b)
+    → "hello world! it's a comment here"
+      by apply Prod.swap
+  (b × a)
+
+@[simp]
+def rev {a} : List a → List a
+  | [] => []
+  | x :: xs => rev xs ++ [x]
+
+structure RevSpec a : Type where
+  fastrev : List a -> List a -> List a
+  correct : ∀ xs ys, rev xs ++ ys = fastrev xs ys
+
+def revCalc {a} : RevSpec a := by
+  calculate fastrev
+  give fastrev by recursion
+  intro xs
+  (induction xs) <;> intro ys
+  case nil => calculator
+      rev [] ++ ys
+    = by rfl
+      ys
+    = by give fastrev [] ys := ys
+      fastrev [] ys
+  case cons x xs ih => calculator
+      rev (x :: xs) ++ ys
+    = by simp only [rev]
+      rev xs ++ [x] ++ ys
+    = by simp only [List.append_assoc]
+      rev xs ++ ([x] ++ ys)
+    = by rfl
+      rev xs ++ x :: ys
+    = by rw [ih]
+      fastrev xs (x :: ys)
+    = by give fastrev (x :: xs) ys := fastrev xs (x :: ys)
+      fastrev (x :: xs) ys
+
+section Compiler
+
+inductive Exp : Type
+  | val : Nat -> Exp
+  | add : Exp -> Exp -> Exp
+  deriving BEq
+
+@[simp]
+def eval : Exp -> Nat
+  | .val n => n
+  | .add x y => eval x + eval y
+
+inductive Code where
+  | push : ℕ → Code → Code
+  | add : Code → Code
+
+abbrev Stack := List Nat
+
+compile_inductive% Exp
+compile_inductive% Code
+open Exp
+open Code
+
+structure CompSpec where
+  comp : Exp -> Code -> Code
+  exec : Code -> Stack -> Stack
+  correct : ∀ e c s, exec c (eval e :: s) = exec (comp e c) s
+
+def comp_calc : CompSpec := by
+  calculate comp, exec
+  give comp by recursion
+  give exec by recursion
+  intro e
+  induction e <;> intros c s
+  case val n => calculator
+      exec c (eval (val n) :: s)
+    = by rfl
+      exec c (n :: s)
+    = by give exec (push n c) s := exec c (n :: s)
+      exec (push n c) s
+    = by give comp (val n) c := push n c
+      exec (comp (val n) c) s
+  case add x y ih_x ih_y => calculator
+      exec c (eval (add x y) :: s)
+    = by rfl
+      exec c ((eval x + eval y) :: s)
+    = by
+        give exec (add c) s by cases of s
+        give exec (add c) (x :: xs) by cases of xs
+        give h : exec (add c) (x :: y :: ys) := exec c ((x + y) :: ys)
+        rw [h]
+        exact []
+        exact []
+      exec (add c) (eval x :: eval y :: s)
+    = by simp only [ih_x]
+      exec (comp x (Code.add c)) (eval y :: s)
+    = by simp only [ih_y]
+      exec (comp y (comp x (Code.add c))) s
+    = by give comp (Exp.add x y) c := comp y (comp x (Code.add c))
+      exec (comp (Exp.add x y) c) s
+
+end Compiler
+
+section Relational
+
+section Syntax
+
+inductive Val where
+  | ofInt : Int -> Val
+  | ofBool : Bool -> Val
+
+instance : Coe Int Val where coe := Val.ofInt
+instance : Coe Nat Val where coe n := Val.ofInt ↑n
+instance : Coe Bool Val where coe := Val.ofBool
+instance {n} : OfNat Val n where ofNat := ↑n
+
+inductive Tm where
+  | ofVal : Val -> Tm
+  | add : Tm -> Tm -> Tm
+  | if_ : Tm -> Tm -> Tm -> Tm
+
+attribute [coe] Val.ofInt
+attribute [coe] Val.ofBool
+attribute [coe] Tm.ofVal
+
+instance : Add Tm where add := Tm.add
+instance : Coe Val Tm where coe := Tm.ofVal
+instance {n} : OfNat Tm n where ofNat := Tm.ofVal ↑n
+
+notation "If " c " then " x " else " y => Tm.if_ c x y
+
+inductive IsVal : Tm -> Prop where
+  | is : IsVal (.ofVal _)
+
+abbrev Value := { x : Tm // IsVal x }
+
+end Syntax
+
+section Semantics
+
+inductive Eval : Tm -> Val -> Prop where
+  | val : {v : Val}
+    -> Eval v v
+  | add : {e e' : Tm} -> {n n' : Int}
+    -> Eval e n -> Eval e' n' -> Eval (e + e') (n + n')
+  | if_t : {e e₁ e₂ : Tm} -> {v : Val}
+    -> Eval e true -> Eval e₁ v -> Eval (If e then e₁ else e₂) v
+  | if_f : {e e₁ e₂ : Tm} -> {v : Val}
+    -> Eval e false -> Eval e₂ v -> Eval (If e then e₁ else e₂) v
+
+scoped infix:60 " ⇓ " => Eval
+
+@[simp, grind .] theorem Eval.rfl {T : Type} [Coe T Val] {v : T} : v ⇓ v := by apply Eval.val
+@[simp, grind .] theorem Eval.rfl.val {v : Val} : v ⇓ v := by apply Eval.val
+@[simp, grind .] theorem Eval.rfl.int {n : Int} : n ⇓ n := by apply Eval.val
+@[simp, grind .] theorem Eval.rfl.nat {n : Nat} : n ⇓ n := by apply Eval.val
+
+end Semantics
+
+section Types
+
+inductive Ty where
+  | Int : Ty
+  | Bool : Ty
+
+inductive HasTy : (v : Val) -> (t : Ty) -> Prop where
+  | isInt : HasTy (.ofInt _) .Int
+  | isBool : HasTy (.ofBool _) .Bool
+
+instance : Membership Val Ty where
+  mem t v := HasTy v t
+
+abbrev TyRel := Tm -> Ty -> Prop
+
+class Sound (rel : TyRel) where
+  soundness : ∀ {e t}, rel e t -> ∃ v, e ⇓ v ∧ v ∈ t
+
+end Types
+
+def semTy : TyRel := fun e t => ∃ v, e ⇓ v ∧ v ∈ t
+scoped notation:50 "⊨ " e:50 " : " t:50 => semTy e t
+
+variable
+  (v v' : Val)
+  (e e' e₁ e₂ : Tm)
+  (t t' : Ty)
+
+end Relational
+
+end Calculator.Example.Alternative
